能量函数: $\mathcal{E}_{g,\lambda,\nu}(\phi) = \lambda\mathcal{L}_{g}(\phi) + \nu \mathcal{A}_g(\phi)$

$\mathcal{L}_{g}(\phi) = \int_{\Omega}g\delta(\phi)\left|\nabla\phi\right|dxdy$            $\mathcal{A}_g(\phi)=\int_{\Omega}gH(-\phi)dxdy$      $g = \frac{1}{1+\left|\nabla G_\sigma * I\right|^2}$

$\delta$ is the univariate Dirac function.

$H$ is the Heaviside function.

演化方程: $\frac{\partial\phi}{\partial t} = \lambda\delta(\phi)div(g\frac{\nabla\phi}{\left|\nabla\phi\right|}) + \nu g\delta(\phi)$

---

My Proof:
$$
\begin{aligned}
\mathcal{E}_{g,\lambda,\nu}(\phi) & = \lambda\mathcal{L}_{g}(\phi) + \nu \mathcal{A}_g(\phi)\\
		& = \lambda\int_{\Omega}g\delta(\phi)\left|\nabla\phi\right|dxdy + \nu\int_{\Omega}gH(-\phi)dxdy\\
		& = \int_{\Omega}\left[\lambda g\delta(\phi)\left|\nabla\phi\right| + \nu gH(-\phi)\right]dxdy 
\end{aligned}
\tag{1}
$$
Let:
$$
F(\phi) = \lambda g\delta(\phi)\left|\nabla\phi\right| + \nu gH(-\phi) \tag{2}
$$

in terms of a small variable $\alpha$ ans an arbitrary function $h$ which satisfies : $h|_{\partial \Omega} = 0$, we can get:
$$
\begin{aligned}
F(\phi+\alpha h) &= \lambda g\delta(\phi+\alpha h)\left|\nabla(\phi+\alpha h)\right| + \nu gH(-(\phi+\alpha h)) \\
                 &= \lambda g\delta(\phi+\alpha h)\sqrt{(\phi + \alpha h)^2_x+(\phi + \alpha h)^2_y}+ \nu gH(-(\phi+\alpha h))
\end{aligned}
\tag{3}
$$

with: 
$$
\delta(\phi) = H'(\phi)\\
\delta(\phi) = \delta(-\phi)
\tag{4}
$$
then:
$$
\begin{aligned}
\frac{\partial F(\phi+\alpha h)}{\partial \alpha} &= \lambda g\left[\delta(\phi+\alpha h)\frac{h_x(\phi+\alpha h)_x + h_y(\phi + \alpha h)_y}{\sqrt{(\phi + \alpha h)^2_x + (\phi + \alpha h)^2_y}} + \\
	h\delta'(\phi+\alpha h)\sqrt{(\phi + \alpha h)^2_x + (\phi + \alpha h)^2_y}  \right] -\nu gH'(-(\phi+\alpha h))\\
	& =  \lambda g\left[\delta(\phi+\alpha h)\frac{h_x(\phi+\alpha h)_x + h_y(\phi + \alpha h)_y}{\sqrt{(\phi + \alpha h)^2_x + (\phi + \alpha h)^2_y}} + \\
	h\delta'(\phi+\alpha h)\sqrt{(\phi + \alpha h)^2_x + (\phi + \alpha h)^2_y}  \right] -\nu g h\delta(\phi+\alpha h)
\end{aligned}
\tag{5}
$$

$$
\begin{aligned}
Then  \frac{\partial F(\phi+\alpha h)}{\partial \alpha}|_{\alpha \rightarrow0} = \lambda g\left[\delta(\phi)\frac{h_x\phi_x + h_y\phi_y}{\sqrt{\phi^2_x + \phi^2_y}} + h\delta'(\phi)\sqrt{\phi^2_x + \phi^2_y}  \right] -\nu g h\delta(\phi) 
\end{aligned}
\tag{6}
$$

Then 
$$
\begin{aligned}
\frac{\partial \mathcal{E}(\phi+\alpha h)}{\partial \alpha}|_{\alpha\rightarrow0} & = \int_{\Omega}\Bigg\lbrace\lambda g\left[\delta(\phi)\frac{h_x\phi_x + h_y\phi_y}{\sqrt{\phi^2_x + \phi^2_y}} + h\delta'(\phi)\sqrt{\phi^2_x + \phi^2_y}  \right] -\nu g h\delta(\phi) \Bigg\rbrace dxdy \\
	& = \int_{\Omega}\Bigg\lbrace\lambda g\left[\delta(\phi)\frac{\nabla\phi\nabla h}{|\nabla\phi|} + h\delta'(\phi)|\nabla\phi|  \right] \Bigg\rbrace dxdy - \int_{\Omega}\nu g h\delta(\phi)dxdy
\end{aligned} 
\tag{7}
$$
According to Green Equation:
$$
\oint_{\partial\Omega} Rdy + Sdx = \iint_{\Omega}(\frac{dS}{dx} - \frac{dR}{dy})dxdy, h|_{\partial \Omega = 0}
\tag{8}
$$
we can get
$$
\begin{aligned}
\int_\Omega g\delta(\phi)\frac{\nabla\phi\nabla h}{|\nabla\phi|}dxdy  &= \int_{\partial \Omega}hg\left[\delta(\phi)\frac{\nabla\phi}{|\nabla\phi|}dy - \delta(\phi)\frac{\nabla\phi}{|\nabla\phi|}dx\right]-\int_\Omega div(g\delta(\phi)\frac{\nabla\phi}{|\nabla\phi|}dxdy \\
	& = -\int_\Omega div(g\delta(\phi)\frac{\nabla\phi}{|\nabla\phi|}dxdy 
\end{aligned}
\tag{9}
$$

Then
$$
\begin{aligned}
\frac{\partial \mathcal{E}(\phi+\alpha h)}{\partial \alpha}|_{\alpha\rightarrow0} &= \int_{\Omega}\Bigg\lbrace\lambda g\left[\delta(\phi)\frac{\nabla\phi\nabla h}{|\nabla\phi|} + h\delta'(\phi)|\nabla\phi|  \right] \Bigg\rbrace dxdy - \int_{\Omega}\nu g h\delta(\phi)dxdy \\
	&= \int_{\Omega}\lambda h\left[g\delta'(\phi)|\nabla\phi|-  div(g\delta(\phi)\frac{\nabla\phi}{|\nabla\phi|}\right]dxdy - \int_{\Omega}\nu g h\delta(\phi)dxdy \\
	&= \int_{\Omega}\lambda h\delta(\phi)(-div(g\frac{\nabla\phi}{|\nabla\phi|})) - \nu g h\delta(\phi)dxdy \\
	&= -\int_{\Omega}h\left[\lambda \delta(\phi)div(g\frac{\nabla\phi}{|\nabla\phi|}) + \nu g\delta(\phi)\right]dxdy 
\end{aligned} 
\tag{10}
$$
When $\mathcal{E}(\phi)$ reach the minimal
$$
\begin{aligned}
\frac{\partial \mathcal{E}(\phi+\alpha h)}{\partial \alpha}|_{\alpha\rightarrow0} &= -\int_{\Omega}\left[\lambda \delta(\phi)div(g\frac{\nabla\phi}{|\nabla\phi|}) + \nu g\delta(\phi)\right]dxdy = 0
\end{aligned} 
\tag{11}
$$
Since function $h$ is arbitrary, we obtain :
$$
\lambda \delta(\phi)div(g\frac{\nabla\phi}{|\nabla\phi|}) + \nu g\delta(\phi) = 0
\tag{12}
$$
Generally, the gradient of functional  $\mathcal{E}_{g,\lambda,\nu}(\phi)$ is denoted as $\{\lambda\delta(\phi)div(g\frac{\nabla\phi}{|\nabla\phi|}) + \nu g\delta(\phi)\}$


 Now we get: $\frac{\partial\phi}{\partial t} = \lambda\delta(\phi)div(g\frac{\nabla\phi}{\left|\nabla\phi\right|}) + \nu g\delta(\phi)$



